iterative hash functions and mismatching types and length indexing oh my

verif/HMAC_specs_equiv.v
@@ -1,13 +1,15 @@
 Require Import List.
 Import ListNotations.
-Require Import Bvector.
 
+Require Import Bvector.
 Require Import Coqlib.
+
+Require Import Utils.
+Require Import Bitstream.
+Require Import Eager.
 
 Require Import HMAC_spec.
 Require Import HMAC_lib.
-Require Import Bitstream.
-Require Import Eager.
 
 
 
@@ -73,10 +75,10 @@ Proof.
 Qed.
 
 (* TODO *)
-Definition correct_model_hash {c p : nat} (hf : ext_val -> ext_val) (h : Bvector (b c p) -> Bvector c) : Prop := True.
+Definition correct_model_hash {c p : nat} (hf : ext_val -> ext_val) (h : list (Bvector (b c p)) -> Bvector c) : Prop := True. 
 
 
-Check HMAC.
+(*Check HMAC.*)
 (* HMAC args in order: c p : nat (bit widths) *)
 (* Bv c -> Bv (c + p) -> Bv c: "compression function", i.e. the hash *)
 (* iv : Bv c "initialization vector" *)
@@ -98,7 +100,30 @@ Definition bv_to_extval {w : nat} (bv : Bvector w) : ext_val :=
   let bits := bv_to_extval' bv in
   let bytes := get_each_n 8 bits in
   eseq (map eseq bytes).
+(*
+Definition get_byte (e : ext_val) : option (list bool) :=
+  match e with
+  | eseq l =>
+    match l with
+    | (ebit b1 :: ebit b2 :: ebit b3 :: ebit b4 ::
+            ebit b5 :: ebit b6 :: ebit b7 :: ebit b8 :: nil) => Some ([b1;b2;b3;b4;b5;b6;b7;b8])
+    | _ => None
+    end
+  | _ => None
+  end.
 
+(* take a list of bytes as an ext_val, convert to flattened bits  *)
+Definition extval_to_bv' (e : ext_val) : option (list bool) :=
+  match e with
+  | eseq l =>
+    match collect (map get_byte l) with
+    | Some bytes =>
+      Some ((fold_left (@app bool) bytes nil))
+    | _ => None
+    end
+  | _ => None
+  end.
+*)
 Lemma split_append :
   forall a (x : Bvector a) b (y : Bvector b),
     splitVector a b (Vector.append x y) = (x,y).
@@ -107,29 +132,72 @@ Proof.
   simpl. reflexivity.
   simpl. rewrite IHx. reflexivity.
 Qed.
-  
+
+
+(*
+Definition extval_to_bv {w : nat} (e : ext_val) :=
+  match extval_to_bv' e with
+  | Some l =>
+    match Nat.eq_dec (length l) w with
+    | left p => Some (Vector.of_list l)
+    | _ => None
+    end
+  | None => None
+  end.
+*)
+
+
 (* I think this is the right theorem *)
 Theorem HMAC_equiv (MSGT : Set) :
   forall keylen msglen key msg,
     has_type key (bytestream keylen) ->
     has_type msg (bytestream msglen) ->
-    forall c p hf res Hash iv (splitAndPad : MSGT -> list (Bvector (b c p))) fpad opad ipad,
+    forall c p hf res HashBlock iv (splitAndPad : MSGT -> list (Bvector (b c p))) fpad opad ipad,
       hmac_model hf key msg = Some res ->
-      @correct_model_hash c p hf (Hash iv) ->
-      forall nmsg nkey nres,
+      @correct_model_hash c p hf (h_star p HashBlock iv) ->
+      forall nmsg nkey,
         eseq (map bv_to_extval (splitAndPad nmsg)) = msg ->
         bv_to_extval nkey = key ->
-        bv_to_extval nres = res ->
-        @HMAC c p Hash iv MSGT splitAndPad fpad opad ipad nkey nmsg = nres.
+        bv_to_extval (@HMAC c p HashBlock iv MSGT splitAndPad fpad opad ipad nkey nmsg) = res.
 Proof.
   intros.
   unfold HMAC.
   unfold HMAC_2K.
   unfold GHMAC_2K.
   unfold hash_words.
-  unfold h_star.
   rewrite split_append.
   simpl. unfold app_fpad.
+  unfold hmac_model in H1.
+  destruct key; simpl in *; try congruence.
+  destruct msg; simpl in *; try congruence.
+  destruct (hf (eseq (map (fun x : ext_val => xor_const 54 x) l ++ l0))) eqn:?; try congruence.
+  inversion H1.
+
+  match goal with
+  | [ |- bv_to_extval (HashBlock (HashBlock iv ?V1) ?V2) = _ ] =>
+    replace (HashBlock (HashBlock iv V1) V2) with (h_star p HashBlock iv (V1 :: V2 :: nil))
+  end.
+  Focus 2. unfold h_star. simpl. reflexivity.
+  match goal with
+  | [ |- context[(h_star p HashBlock (HashBlock iv ?V1) ?V2)] ] =>
+    replace (h_star p HashBlock (HashBlock iv V1) V2) with (h_star p HashBlock iv (V1 :: V2))
+  end.
+  Focus 2. simpl. reflexivity.
+  remember (h_star p HashBlock iv) as HASH.
+
+  
+  
+  (* TODO: What's the correct version of this? *)
+Lemma correct_hash_commutes :
+  forall {n m} h (hf : Bvector n -> Bvector (b n m) -> Bvector n) iv,
+    correct_model_hash h hf iv ->
+    forall x y,
+      @bv_to_extval n (hf x y) = h (@bv_to_extval (b n m) y).
+Proof.
+Admitted.
+
+
+
   
   
 Admitted.
